

Analysis I Homework 5+

A. Prove Arithmetic of Infinity Limits, part (iii).

$(r_n), (s_n) \Rightarrow$ real sequences

$$\lim_{n \rightarrow \infty} r_n = r$$

$$\lim_{n \rightarrow \infty} s_n = \infty$$

For $r > 0 \Rightarrow \lim_{n \rightarrow \infty} (r_n + s_n) = +\infty$, and for $r < 0 \Rightarrow \lim_{n \rightarrow \infty} (r_n + s_n) = -\infty$.

If $\lim_{n \rightarrow \infty} r_n = r \Leftrightarrow \forall \epsilon > 0 \exists n_\epsilon \in \mathbb{N} \forall n > n_\epsilon |r_n - r| < \epsilon \Leftrightarrow r - \epsilon < r_n < r + \epsilon$,

$\lim_{n \rightarrow \infty} s_n = \infty \Leftrightarrow \forall N > 0 \exists n_2 \forall n > n_2 s_n > N$ and $r > 0$. Then $M > 0$

$n_M = \max\{n_\epsilon, n_2\}$ and $n > n_M$

$$\Rightarrow \lim_{n \rightarrow \infty} (r_n + s_n) = +\infty \quad \blacksquare$$

B. Explain why if a_n converges, then $\lim_{n \rightarrow \infty} a_n = \lim_{n \rightarrow \infty} a_{n+1}$.

$$\text{If } \lim_{n \rightarrow \infty} a_n = L \Rightarrow \lim_{n \rightarrow \infty} a_{n+1} = L$$

$$\text{For } \lim_{n \rightarrow \infty} a_n = L \Leftrightarrow \forall \epsilon > 0, \exists N \in \mathbb{N} \text{ s.t. } n > N \Rightarrow |a_n - L| < \epsilon$$

$$c_n = a_{n+1} \text{ where } n = 1, 2, \dots$$

$$\epsilon > 0 \quad \exists N_0 = N_\epsilon - 1 \text{ and } n > N_0$$

$$|c_n - L| = |a_{n+1} - L| < \epsilon$$

$$\Leftrightarrow n+1 > N_\epsilon$$

$$\Leftrightarrow n > N_\epsilon - 1$$

$$\Rightarrow \lim_{n \rightarrow \infty} c_n = L = \lim_{n \rightarrow \infty} a_{n+1}$$

C. Let $r > 0$ be a positive real number. This problem will give a simple approach to $\lim_{n \rightarrow \infty} r^n$.

(i) Explain briefly why $a_n = r^n$ can be written recursively as $a_0 = 1, a_n = r \cdot a_{n-1}$ for $n > 0$.

(ii) Using problem A and (i), solve for the possible limits of a_n if the sequence converges.

(iii) Show that a_n is monotone. (It may be increasing or decreasing, depending on r .)

(iv) Combine (ii) and (iii) to show $\lim_{n \rightarrow \infty} r^n$ converges to 0 for $r < 1$, converges to 1 for $r = 1$, and diverges to ∞ for $r > 1$.

(i) $a_n = r^n, r > 0$ Recursively written $a_0 = 1, a_n = r \cdot a_{n-1}, n > 0$

Proof: 1) $n=0 \quad a_0 = r^0 = a_0 = 1$

2) If it's true that $n=k, a_k = r^k, a_k = r \cdot a_{k-1}$

3) We should prove $n=k+1, a_{k+1} = r^{k+1} \quad a_{k+1} = r \cdot a_k$

$$\Rightarrow a_{k+1} = r \cdot a_k = r \cdot r^k = r^{k+1} \quad \blacksquare$$

(ii) $\lim_{n \rightarrow \infty} a_n = \lim_{n \rightarrow \infty} (r \cdot a_{n-1})$

$$r=1 \quad \lim_{n \rightarrow \infty} a_n = \lim_{n \rightarrow \infty} 1^n = 1$$

$$0 < r < 1 \quad \lim_{n \rightarrow \infty} a_n = \lim_{n \rightarrow \infty} r \cdot a_{n-1} = r \cdot \lim_{n \rightarrow \infty} a_{n-1}$$

$$L = r \cdot L$$

$$(1-r) \neq 0 \quad L=0$$

$\Rightarrow L=0$ if converges

(iii) $0 < r < 1$

$$a_n = r^n$$

$$\frac{a_{n+1}}{a_n} = \frac{r^{n+1}}{r^n} = r < 1 \quad (a_n) \downarrow$$

If $r > 1$

$$\frac{a_{n+1}}{a_n} = \frac{r^{n+1}}{r^n} = r > 1 \quad (a_n) \uparrow$$

$$\left. \begin{array}{l} \text{(iv) } a_n = r^n \quad (a_n) \downarrow \\ 0 < r < 1 \Rightarrow 0 < r^n \end{array} \right\} \Leftrightarrow \exists \lim_{n \rightarrow \infty} a_n = L \Rightarrow a_n = r \cdot a_{n-1} \quad / \quad \exists \lim_{n \rightarrow \infty} a_{n-1}$$

$$\lim_{n \rightarrow \infty} a_n = r \lim_{n \rightarrow \infty} a_{n-1}$$

$$L = r \cdot L$$

$$(1-r)L = 0$$

$$\Rightarrow L = 0$$

$r > 1 \quad (a_n) \nearrow$ it is not bounded

$$\Rightarrow \lim_{n \rightarrow \infty} a_n = \infty$$

D. Consider the recursively defined sequence $S_1 = 1$ and $S_{n+1} = 1/(4 - S_n)$ for $n \geq 1$.

(i) Prove that S_n converges. (Hint: is the sequence monotone?)

(ii) Solve to find the limit.

$$(i) \quad S_1 = 1, \quad S_2 = \frac{1}{4 - S_1} = \frac{1}{4 - 1} = \frac{1}{3}$$

$$S_3 = \frac{1}{4 - S_2} = \frac{1}{4 - \frac{1}{3}} = \frac{3}{11}, \quad S_4 = \frac{1}{4 - S_3} = \frac{1}{4 - \frac{3}{11}} = \frac{11}{41}$$

$$S_1 = 1 > S_2 = \frac{1}{3} > S_3 = \frac{3}{11} > S_4 = \frac{11}{41}$$

I will prove that (S_n) is bounded from below

$$S_n \geq 2 - \sqrt{3} \quad \forall n \in \mathbb{N}$$

$$1^\circ \quad n=1 \quad S_1 = 1 \geq 2 - \sqrt{3} = 0, \dots$$

$$2^\circ \quad n=k \quad S_k \geq 2 - \sqrt{3}$$

$$3^\circ \quad \text{For } n=k+1 \Rightarrow S_{k+1} \geq 2 - \sqrt{3}$$

$$S_{k+1} \geq 2 - \sqrt{3} \Leftrightarrow \frac{1}{4 - S_k} \geq 2 - \sqrt{3} \Leftrightarrow 1 \geq 8 - 4\sqrt{3} - (2 - \sqrt{3})S_k \Leftrightarrow$$

$$\Leftrightarrow (2 - \sqrt{3})S_k \geq 7 - 4\sqrt{3} \quad \Leftrightarrow S_k \geq \frac{7 - 4\sqrt{3}}{2 - \sqrt{3}} \cdot \frac{2 + \sqrt{3}}{2 + \sqrt{3}} \Leftrightarrow$$

$$\Leftrightarrow S_k \geq \frac{14 - 8\sqrt{3} + 4\sqrt{3} - 12}{4 - 3} = 2 - \sqrt{3}$$

$$(ii) \quad (S_n) \downarrow \quad \forall n \quad S_{n+1} \leq S_n$$

$$1^\circ \quad S_2 = \frac{1}{3} \leq S_1 = 1$$

$$2^\circ \quad n=k, \quad S_{k+1} \leq S_k$$

$$3^\circ \quad n=k+1 \quad S_{k+2} \leq S_{k+1}$$

$$\Leftrightarrow \frac{1}{4 - S_{k+1}} \leq \frac{1}{4 - S_k} \Leftrightarrow 4 - S_k \leq 4 - S_{k+1} \quad \Leftrightarrow -S_k \leq -S_{k+1} \quad \Leftrightarrow$$

$$\Leftrightarrow S_k \geq S_{k+1}$$

From (i)+(ii) $\Rightarrow \exists L = \lim_{n \rightarrow \infty} S_n$

$$S_{n+1} = \frac{1}{4 - S_n} \quad \bigg/ \quad \lim_{n \rightarrow \infty}$$

$$\Leftrightarrow L = \frac{1}{4 - L} \Leftrightarrow 4L - L^2 = 1 \Leftrightarrow 0 = L^2 - 4L + 1 \Leftrightarrow$$

$$\Leftrightarrow L_{1/2} = \frac{4 \pm \sqrt{16 - 4}}{2} = 2 \pm \sqrt{3}$$

$$L_1 = 2 - \sqrt{3} \quad L_2 = 2 + \sqrt{3}$$

E. Working directly from the definition (and without using Cauchy Completeness Theorem), show any Cauchy sequence of real numbers is bounded.

(a_n) is Cauchy sequence

$$\forall \epsilon > 0 \quad \exists n_0 \quad \forall n, m > n_0 \quad |a_n - a_m| < \epsilon$$

$$\exists n_1 \quad \forall n, m > n_1 \quad |a_n - a_m| < 1$$

$$m = n_n + 1 \quad |a_n - a_{n+1}| < 1$$

If $n > n_1$

$$|a_n| = |a_n - a_{n+1} + a_{n+1}| \leq |a_n - a_{n+1}| + |a_{n+1}| < 1 + |a_{n+1}|$$

$$M = \max \{ |a_1|, |a_2|, \dots, |a_{n_1}|, |a_{n_1+1}| + 1 \}$$

$$\Rightarrow \forall n \in \mathbb{N} \quad |a_n| < M$$

$\Rightarrow (a_n)$ is bounded

F. Make an educated guess as to the limit of the complex sequence $z_n = i^n / (2n+6)$. Working directly from the definition of complex limit, show that your answer is correct.

$$z_n = \frac{i^n}{2n+6} = \begin{cases} \frac{1}{2n+6}, & n=4k \\ \frac{i}{2n+6}, & n=4k+1 \\ \frac{-1}{2n+6}, & n=4k+2 \\ \frac{-i}{2n+6}, & n=4k+3 \end{cases}$$

$$\Rightarrow \lim_{n \rightarrow \infty} z_n = 0$$

G. Let S_n be bounded sequence, and let t_n converge to L .

(i) Show that if $L=0$, then the product $S_n \cdot t_n$ also converges to 0.

(ii) Give an example where S_n is bounded and t_n converges, but where the product does not converge.

Hint: One approach to (i) uses Sandwich Theorem.

$$(i) |S_n| < M \quad \forall n \in \mathbb{N} \quad (-M < S_n < M)$$

$$\lim_{n \rightarrow \infty} t_n = 0$$

$$\lim_{n \rightarrow \infty} S_n \cdot t_n = 0$$

$$a_n = -M \cdot t_n \leq S_n \cdot t_n \leq M \cdot t_n = b_n$$

$$\lim_{n \rightarrow \infty} a_n = \lim_{n \rightarrow \infty} (-M \cdot t_n) = -M \lim_{n \rightarrow \infty} t_n = -M \cdot 0 = 0$$

$$\lim_{n \rightarrow \infty} b_n = \lim_{n \rightarrow \infty} (M \cdot t_n) = M \lim_{n \rightarrow \infty} t_n = M \cdot 0 = 0$$

$$\Rightarrow \lim_{n \rightarrow \infty} (S_n \cdot t_n) = 0$$

$$(ii) \text{ If } S_n = \cos n\pi$$

$$|S_n| \leq 1 \quad \forall n \in \mathbb{N}$$

$$t_n = \frac{n}{n+1} \quad \lim_{n \rightarrow \infty} t_n = 1$$

$$a_n = S_n \cdot t_n = \cos n\pi \cdot \frac{n}{n+1} = \begin{cases} \frac{n}{n+1} & , n=2k \\ \frac{-n}{n+1} & , n=2k+1 \end{cases}$$

$$a_{2k} = \frac{n}{n+1} \rightarrow 1$$

$$a_{2k+1} = \frac{-n}{n+1} \rightarrow -1$$

$$\Rightarrow \nexists \lim_{n \rightarrow \infty} a_n$$